theories/typing/lib/ghostptrtoken/ghostseq_basic.v
@@ -1,6 +1,6 @@
 From lrust.util Require Export pairwise.
 From lrust.typing Require Export type.
-From lrust.typing Require Import array_util typing logic_fn always_true.
+From lrust.typing Require Import array_util typing ghost_fn always_true.
 From lrust.typing.lib.ghostptrtoken Require Export ghostseq.
 From stdpp Require Import numbers.
 Set Default Proof Using "Type".
@@ -303,7 +303,7 @@ Section ghostseq_basic.
   Proof.
     eapply tctx_incl_ext. eapply tctx_incl_trans. eapply tctx_incl_tail. eapply copy_ghost. done. apply ghost_copy.
     eapply tctx_incl_trans. eapply (tctx_incl_app +[_; _] _ +[_] _). apply seq_split.
-    eapply (logic_fn_ghost_tctx_incl' [p2] _ +[]). eapply (plain_logic_fn +[_] _ (λ '-[x], (1: Zₛ))).
+    eapply (logic_fn_ghost_tctx_incl' [p2] _ +[] int (const 1)). eapply (plain_ghost_fn (𝔅:=Zₛ) +[_]).
     eapply tctx_incl_trans. eapply tctx_incl_tail. eapply tctx_incl_trans. apply seq_split.
     eapply tctx_incl_trans. apply tctx_incl_swap. eapply tctx_incl_tail. apply seq_destruct_singleton. done.
     eapply (tctx_incl_frame_r +[_; _] +[_]). eapply seq_append.
